Use lists for the context, not sets
This also makes more sense because it does not require us to have unique
variable identifiers but represents variable shadowing just like the one
present in most programming languages

Soundness.thy
@@ -2,8 +2,8 @@ theory Soundness
   imports Defs
 begin
 
-theorem progress: "{} \<turnstile> e : \<tau> \<Longrightarrow> is_v_of_e e \<or> (\<exists>e'. Step e e')"
-proof (induction "{} :: \<Gamma>" e \<tau> rule: T.induct)
+theorem progress: "[] \<turnstile> e : \<tau> \<Longrightarrow> is_v_of_e e \<or> (\<exists>e'. Step e e')"
+proof (induction "[] :: \<Gamma>" e \<tau> rule: T.induct)
   case T_UnitI
   then show ?case by simp
 next
@@ -23,7 +23,8 @@ next
     from IH2 show ?thesis
     proof (elim disjE)
       assume "is_v_of_e e2"
-      from \<open>is_v_of_e e1\<close> T_AppI have "\<exists>x e. e1 = (\<lambda>x:\<tau>1. e)" by (metis T.cases \<tau>.inject \<tau>.simps(3) empty_iff is_v_of_e.simps(3))
+      from \<open>is_v_of_e e1\<close> T_AppI have "\<exists>x e. e1 = (\<lambda>x:\<tau>1. e)"
+        by (metis T.cases \<tau>.distinct(1) \<tau>.inject is_v_of_e.simps(1) is_v_of_e.simps(3))
       then have "\<exists>e'. Step (App e1 e2) e'" using \<open>is_v_of_e e2\<close> ST_BetaI by blast
       then show ?thesis by simp
     next
@@ -38,18 +39,13 @@ next
   qed
 qed
 
-definition fve :: "e \<Rightarrow> x set" where
-  "fve e \<equiv> set (fve_e e)"
-
 definition closed :: "e \<Rightarrow> bool" where
-  "closed x \<equiv> fve x = {}"
-
-declare fve_def[simp]
+  "closed x \<equiv> fve_e x = []"
 
 lemma list_minus_set: "set (list_minus e xs) = set e - set xs"
   by (induction e) (auto)
 
-lemma free_in_context: "\<lbrakk> x \<in> fve e ; \<Gamma> \<turnstile> e : \<tau> \<rbrakk> \<Longrightarrow> \<exists>\<tau>'. (x, \<tau>') \<in> \<Gamma>"
+lemma free_in_context: "\<lbrakk> x \<in> set (fve_e e) ; \<Gamma> \<turnstile> e : \<tau> \<rbrakk> \<Longrightarrow> \<exists>\<tau>'. (x, \<tau>') \<in> \<Gamma>"
 proof (induction e arbitrary: \<Gamma> \<tau> x)
   case (Var y)
   then show ?case using T.cases by fastforce
@@ -58,20 +54,21 @@ next
   then have "x \<noteq> y" by (simp add: list_minus_set)
   then have "x \<in> set (fve_e e)" using list_minus_set T.cases Lam by fastforce
   then show ?case
-    by (metis fve_def Lam.IH Lam.prems(2) T.cases \<open>x \<noteq> y\<close> e.distinct(9) e.inject(2) e.simps(11) e.simps(5) insertE prod.inject)
+    by (metis (no_types, lifting) Lam(3) Lam.IH T.cases \<open>x \<noteq> y\<close> e.distinct(1) e.distinct(9) e.simps(11) e.simps(2) isin.simps(2))
 next
   case (App e1 e2)
-  then show ?case by (metis fve_def T.cases Un_iff e.simps(11) e.simps(15) e.simps(3) e.simps(7) fve_e.simps(3) set_append)
+  then show ?case
+    by (metis (no_types, lifting) T.cases UnE e.distinct(11) e.distinct(3) e.distinct(7) e.inject(3) fve_e.simps(3) set_append)
 next
   case Unit
   then show ?case by simp
 qed
 
-corollary typeable_closed: "{} \<turnstile> e : \<tau> \<Longrightarrow> closed e"
-  unfolding closed_def fve_def
+corollary typeable_closed: "[] \<turnstile> e : \<tau> \<Longrightarrow> closed e"
+  unfolding closed_def
   using free_in_context last_in_set by fastforce
 
-lemma context_invariance: "\<lbrakk> \<Gamma> \<turnstile> e : \<tau> ; \<forall>(x, \<tau>')\<in>\<Gamma>. x\<in>fve e \<longrightarrow> (x, \<tau>')\<in>\<Gamma>' \<rbrakk> \<Longrightarrow> \<Gamma>' \<turnstile> e : \<tau>"
+lemma context_invariance: "\<lbrakk> \<Gamma> \<turnstile> e : \<tau> ; \<forall>x \<tau>'. x \<in> set (fve_e e) \<and> (x, \<tau>') \<in> \<Gamma> \<longrightarrow> (x, \<tau>')\<in>\<Gamma>' \<rbrakk> \<Longrightarrow> \<Gamma>' \<turnstile> e : \<tau>"
 proof (induction \<Gamma> e \<tau> arbitrary: \<Gamma>' rule: T.induct)
   case (T_UnitI \<Gamma>)
   then show ?case by (simp add: T.T_UnitI)
@@ -80,29 +77,24 @@ next
   then show ?case by (auto simp: T.T_VarI)
 next
   case (T_AbsI y \<tau>1 \<Gamma> e \<tau>2)
-  have fresh: "y # \<Gamma>'" sorry
-
-  have "\<forall>(x, \<tau>')\<in>insert (y, \<tau>1) \<Gamma>. x \<in> fve e \<longrightarrow> (x, \<tau>') \<in> insert (y, \<tau>1) \<Gamma>" by blast
-  then have "insert (y, \<tau>1) \<Gamma>' \<turnstile> e : \<tau>2" using T_AbsI(3)[of "insert (y, \<tau>1) \<Gamma>"]
-    by (smt Diff_iff T_AbsI.IH T_AbsI.hyps(2) T_AbsI.prems case_prodD case_prodI2 empty_iff fresh.elims(2) fve_def fve_e.simps(2) insert_iff list.set(1) list.simps(15) list_minus_set)
-  then show ?case using T.T_AbsI[of y \<tau>1 \<Gamma>' e \<tau>2] T_AbsI fresh by simp
+  then show ?case by (simp add: T.T_AbsI list_minus_set)
 next
   case (T_AppI \<Gamma> e1 \<tau>1 \<tau>2 e2)
-  then show ?case apply (auto split: prod.splits) by (metis (mono_tags, lifting) T.T_AppI case_prodI2)
+  then show ?case by auto (metis (mono_tags, lifting) T.T_AppI)
 qed
 
-lemma substitution: "\<lbrakk> insert (x, \<tau>') \<Gamma> \<turnstile> e : \<tau> ; {} \<turnstile> v : \<tau>' ; x # \<Gamma> \<rbrakk> \<Longrightarrow> \<Gamma> \<turnstile> esubst_e v x e : \<tau>"
-proof (induction "insert (x, \<tau>') \<Gamma>" e \<tau> arbitrary: v x \<tau>' \<Gamma> rule: T.induct)
+lemma substitution: "\<lbrakk> (x, \<tau>')#\<Gamma> \<turnstile> e : \<tau> ; [] \<turnstile> v : \<tau>' \<rbrakk> \<Longrightarrow> \<Gamma> \<turnstile> esubst_e v x e : \<tau>"
+proof (induction "(x, \<tau>')#\<Gamma>" e \<tau> arbitrary: v x \<tau>' \<Gamma> rule: T.induct)
 case T_UnitI
   then show ?case by (simp add: T.T_UnitI)
 next
   case (T_VarI y \<sigma>)
-  then have t: "insert (x, \<tau>') \<Gamma> \<turnstile> Var y : \<sigma>" using T.T_VarI by simp
+  then have t: "(x, \<tau>')#\<Gamma> \<turnstile> Var y : \<sigma>" using T.T_VarI by simp
   then show ?case
   proof (cases "y = x")
     case True
     then have "\<sigma> = \<tau>'" using T_VarI by fastforce
-    then show ?thesis using context_invariance T_VarI.prems(1) True by auto
+    then show ?thesis using T_VarI.prems True context_invariance by fastforce
   next
     case False
     then have "\<Gamma> \<turnstile> Var y : \<sigma>" using t T.T_VarI T_VarI.hyps by auto
@@ -115,9 +107,9 @@ next
   proof (cases "x = y")
     case True
     then have same: "esubst_e v x ?lam = ?lam" using T_AbsI by simp
-    then have fv: "x \<notin> fve ?lam" by (simp add: list_minus_set True)
-    then have "insert (x, \<tau>') \<Gamma> \<turnstile> ?lam : \<tau>1 \<rightarrow> \<tau>2" using T.T_AbsI T_AbsI by simp
-    then have "\<Gamma> \<turnstile> ?lam : \<tau>1 \<rightarrow> \<tau>2" using True fv context_invariance by blast
+    then have fv: "x \<notin> set (fve_e ?lam)" by (simp add: list_minus_set True)
+    then have "(x, \<tau>')#\<Gamma> \<turnstile> ?lam : \<tau>1 \<rightarrow> \<tau>2" using T.T_AbsI T_AbsI by simp
+    then have "\<Gamma> \<turnstile> ?lam : \<tau>1 \<rightarrow> \<tau>2" using fv context_invariance by auto
     then show ?thesis using same by simp
   next
     case False
